\documentclass[12pt]{jsarticle}
\usepackage{amsmath,amssymb}
\pagestyle{empty}
\begin{document}
\setlength{\baselineskip}{22pt}
\begin{flushleft}
{\huge 4}
　$n$を正の整数とし，$n$次の整式$P_n(x)=x(x+1)\cdots(x+n-1)$を展開して
$\displaystyle P_n(x)=\sum_{m=1}^n {}_nB_m x^m$と表す。
\begin{description}
\item[(1)]等式$\displaystyle \sum_{m=1}^n {}_nB_m = n \, !$を示せ。
\item[(2)]等式
\[ P_n(x+1)=\sum_{m=1}^n( {}_nB_m \cdot {}_mC_0 + {}_nB_m \cdot {}_mC_1 x + \cdots +
{}_nB_m \cdot {}_mC_m x^m ) \]
を示せ。ただし，${}_mC_0, \, {}_mC_1, \, \cdots, \, {}_mC_m$は二項係数である。
\item[(3)]$k=1, \, 2, \, \cdots, \, n$に対して，
等式$\displaystyle \sum_{j=k}^n {}_nB_j \cdot {}_jC_k = {}_{n+1}B_{k+1} $を示せ。
\end{description}
\end{flushleft}
\end{document}
