\documentclass[12pt]{jsarticle}
\usepackage{amsmath,amssymb}
\pagestyle{empty}
\begin{document}
\setlength{\baselineskip}{22pt}
\begin{flushleft}
{\huge 3}
　数列$\{ a_n \}$を次の条件により定める。
\[ a_1=1, \hspace{1zw} a_2=3, \]
\[ (n+1)a_{n+2}-(2n+3)a_{n+1}+(n+2)a_n=0 \hspace{1zw} (n=1, \, 2, \, 3, \, \cdots\cdots) \]
\begin{description}
\item[(1)]$b_n=a_{n+1}-a_n$とおくと，
\[ b_{n+1}=\frac{n+2}{n+1}b_n \hspace{1zw} (n=1, \, 2, \, 3, \, \cdots\cdots) \]
が成り立つことを示せ。
\item[(2)]数列$\{ a_n \}$の一般項を求めよ。
\item[(3)]$\displaystyle\sum_{n=1}^{225}\frac{1}{a_n}$の値を求めよ。
\end{description}
\end{flushleft}
\end{document}
