\documentclass[12pt]{jsarticle}
\usepackage{amsmath,amssymb}
\pagestyle{empty}
\begin{document}
\setlength{\baselineskip}{22pt}
\begin{flushleft}
{\huge 4}
　数列$a_0, \, a_1, \, a_2, \, \cdots\cdots, \, a_n, \, \cdots\cdots$は
$4{a_{n+1}}^3+3a_{n+1}-a_n=0$ $(n=0, \, 1, \, 2, \, \cdots\cdots)$を満たすとし，
$\displaystyle S_n=\sum_{k=1}^n3^{k-1}{a_k}^3$ $(n=1, \, 2, \, 3, \, \cdots\cdots)$とおく．
ただし，$a_0\neq0$とする．
\begin{description}
\item[(1)]すべての自然数$n$に対して，
$\displaystyle S_n=-\frac{3^n}{4}a_n+\frac{1}{4}a_0$が成り立つことを数学的帰納法で示せ．
\item[(2)]$\displaystyle f(x)=\frac{e^x-e^{-x}}{2}$（$e$は自然対数の底）とし，
数列$x_0, \, x_1, \, x_2, \, \cdots\cdots, \, x_n, \, \cdots\cdots$は
$a_n=f(x_n)$を満たすとする．
$x_n$を$x_0$で表せ．
\item[(3)]$\displaystyle\lim_{n\to\infty}S_n$を$x_0$で表せ．
\end{description}
\end{flushleft}
\end{document}
