\documentclass[12pt]{jsarticle}
\usepackage{amsmath,amssymb}
\pagestyle{empty}
\begin{document}
\setlength{\baselineskip}{22pt}
\begin{flushleft}
{\huge 3}
　$\displaystyle g(x)=\frac{e^{2x}-1}{e^{2x}+1}$，
$\displaystyle f(x)=\frac{g(a)+x}{1+g(a)x}$とする．
ただし，$a$は定数，$e$は自然対数の底である．
\begin{description}
\item[(1)]すべての実数$t$に対して，$f(g(t))=g(t+a)$を示せ．
\item[(2)]$x_1=g(a)$，$x_{n+1}=f(x_n)$ $(n=1, \, 2, \, 3, \, \cdots\cdots)$により
数列$\{ x_n \}$を定める．
$a>0$として，$\displaystyle\lim_{n\to\infty}x_n$を求めよ．
\end{description}
\end{flushleft}
\end{document}
