\documentclass[12pt]{jsarticle}
\usepackage{amsmath,amssymb}
\pagestyle{empty}
\begin{document}
\setlength{\baselineskip}{22pt}
\begin{flushleft}
{\huge 1}
　2つの数列$\{ a_k \}$，$\{ b_k \}$をそれぞれ
\[ a_k=\frac{1}{k \, !} \hspace{1zw} (k=1, \, 2, \, \cdots\cdots) \]
\[ b_k=\frac{1}{k(k+1)} \hspace{1zw} (k=1, \, 2, \, \cdots\cdots) \]
と定める．また，$n=1, \, 2, \, \cdots\cdots$に対して
\[ s_n=\sum_{k=1}^n{(-1)}^ka_k, \hspace{1zw} t_n=\sum_{k=1}^nb_k, \hspace{1zw} u_n=\sum_{k=1}^na_k \]
とおく．このとき，任意の$n$について，次の(1)，(2)，(3)を証明せよ．
\begin{description}
\item[(1)]$s_n<0$
\item[(2)]$t_n<1$
\item[(3)]$u_n<2$
\end{description}
\end{flushleft}
\end{document}
