\documentclass[12pt]{jsarticle}
\usepackage{amsmath,amssymb}
\pagestyle{empty}
\begin{document}
\setlength{\baselineskip}{22pt}
\begin{flushleft}
{\huge 3 (a)}
　数列$\{ a_n \}$から，関係式
\[ b_1=a_1, \hspace{1zw} b_2=a_2-\frac{1}{1 \, !}a_1, \]
\[ \cdots\cdots\cdots\cdots\cdots \]
\[ b_n=a_n-\frac{1}{1 \, !}a_{n-1}+\frac{1}{2 \, !}a_{n-2}-\cdots+{(-1)}^{n-1}\frac{1}{(n-1) \, !}a_1, \]
\[ \cdots\cdots\cdots\cdots\cdots \]
によって数列$\{ b_n \}$を定めるとき，次の(1)，(2)を解答せよ．
\begin{description}
\item[(1)]$\displaystyle a_1=1, \, a_2=\frac{1}{1 \, !}, \, \cdots\cdots, \, a_n=\frac{1}{(n-1) \, !}, \, \cdots\cdots$ならば
$b_1=1$，$b_n=0$ $(n=2, \, 3, \, \cdots\cdots)$である．
\item[(2)]$\displaystyle a_1=1, \, a_2=a_1+\frac{1}{1 \, !}, \, \cdots\cdots, \,
a_n=a_{n-1}+\frac{1}{(n-1) \, !}, \, \cdots\cdots$ならば$b_n=1$ $(n=1, \, 2, \, \cdots\cdots)$である．
\end{description}
\end{flushleft}
\end{document}
