\documentclass[12pt]{jsarticle}
\usepackage{amsmath,amssymb}
\pagestyle{empty}
\begin{document}
\setlength{\baselineskip}{22pt}
\begin{flushleft}
{\huge 2}
　次の条件によって定められる数列$\{ a_n \}$がある．
\[ a_1=1, \hspace{1zw} a_{n+1}=\frac{2n-1}{2n}a_n \hspace{1zw} (n=1, \, 2, \, 3, \, \cdots) \]
\begin{description}
\item[(1)]正の整数$k, \, l$に対して
\[ \frac{k}{k+l-1}a_{k+1}a_l+\frac{l}{k+l-1}a_ka_{l+1}=a_ka_l \]
が成り立つことを示せ．
\item[(2)]正の整数$m$に対して
\[ \sum_{k=1}^ma_ka_{m-k+1}=1 \]
が成り立つことを示せ．
\end{description}
\end{flushleft}
\end{document}
