\documentclass[12pt]{jsarticle}
\usepackage{amsmath,amssymb}
\pagestyle{empty}
\begin{document}
\setlength{\baselineskip}{22pt}
\begin{flushleft}
{\huge 1}
　2つの数列$\{ a_n \}$，$\{ b_n \}$は，条件
\begin{description}
\item[（イ）]$\displaystyle\sum_{k=1}^{2n}{(-1)}^{k-1}a_k=
\sum_{l=1}^n\frac{b_l}{n+l}$ $(n=1, \, 2, \, \cdots\cdots)$
\item[（ロ）]$\displaystyle 0<a_n\leqq\frac{1}{n}$ $(n=1, \, 2, \, \cdots\cdots)$
\item[（ハ）]$b_n$ $(n=1, \, 2, \, \cdots\cdots)$は正の整数
\end{description}
を満たすものとする．\\
　次の問に答えよ．
\begin{description}
\item[(1)]$b_1=1$を示せ．
\item[(2)]$b_n$ $(n=2, \, 3, \, \cdots\cdots)$を求めよ．
\item[(3)]さらに$\{ a_n \}$が$\displaystyle a_{2n}=\frac{1}{2}a_n$ $(n=1, \, 2, \, \cdots\cdots)$を
満たすとき，$a_n$ $(n=1, \, 2, \, \cdots\cdots)$を求めよ．
\end{description}
\end{flushleft}
\end{document}
